TypeSystem.v
@@ -466,7 +466,6 @@ Lemma ty_sound_closure:
     TcRho (rho, rgns) -> 
     TcEnv (stty, rho, env, ctxt) ->
     TcExp (ctxt, rgns,  Mu f x ec ee, Ty2_Arrow tyx effc tyc effe Ty2_Effect, Empty_Static_Action) -> 
-    (forall r : Name, r # subst_rho rho (Ty2_Arrow tyx effc tyc effe Ty2_Effect)) ->
     TcVal (stty, Cls (env, rho,  Mu f x ec ee),  subst_rho rho (Ty2_Arrow tyx effc tyc effe Ty2_Effect)).   
 Proof.
   intros; econstructor; eauto.
@@ -477,8 +476,6 @@ Lemma ty_sound_region_closure:
     TcRho (rho, rgns) -> 
     TcEnv (stty, rho, env,ctxt) ->
     TcExp (ctxt, rgns, Lambda x er, Ty2_ForallRgn (close_var_eff x effr) (close_var x tyr),  Empty_Static_Action) ->
-    (forall r : Name,
-       r # subst_rho rho (Ty2_ForallRgn (close_var_eff x effr) (close_var x tyr))) ->
     TcVal (stty, Cls (env, rho, Lambda x er), subst_rho rho (Ty2_ForallRgn (close_var_eff x effr) (close_var x tyr))).
 Proof.
   intros. econstructor; eauto.
@@ -509,33 +506,6 @@ Proof.
   apply H2. 
   eapply H0; eassumption.
 Qed.  
-
-Lemma subst_rho_close_var:
-  forall x x0 rho tyr,
-    R.find (elt:=nat) x rho = None ->
-    In Name (frv (subst_rho rho (close_var x tyr))) x0 ->
-    In Name (frv (close_var x tyr)) x0.
-Proof. 
-  intros.  
-  destruct rho; induction this.
-  - clear H. unfold In. unfold subst_rho, R.fold in H0; simpl in H0. assumption.
-  - inversion is_bst; subst.  
-    eapply frv_in_subst_rho in H0.
-    destruct H0. 
-    + eapply IHthis1. 
-      * eapply find_rho_1; eauto.
-      * unfold In. assumption.
-    + destruct H0. 
-      * unfold In. unfold subst_in_type in H0.
-        assert (k # (close_var x tyr)) by admit.
-        assert ([k := Rgn2_Const true false e] close_var x tyr = close_var x tyr).
-        apply SUBST_FRESH; auto.
-        rewrite H2 in H0.
-        assumption.
-      * eapply IHthis2; eauto.
-        eapply find_rho_2; eauto.  
-    Unshelve. auto. auto. auto. auto.
-Admitted.
 
 Lemma ty_sound:
   forall e env rho hp hp' v dynamic_eff,
@@ -568,29 +538,15 @@ Proof.
     eapply ty_sound_closure; try (solve [eassumption]). auto.
   Case "rgn_abs". 
     exists stty;  (split; [| split]; auto). 
-    eapply ty_sound_region_closure; try (solve [eassumption]). 
-    rewrite subst_rho_forallrgn. intro. simpl.
-    simpl in H8. 
-    assert (R.find (elt:=nat) x rho = None) by 
-        (inversion Hrho; eapply contrapositiveTcRho; eauto).
-    unfold not_set_elem, Complement in *. intuition.
-    destruct H0.  
-    SCase "case1".
-      apply H8 with  (r:=x0). unfold In in *; simpl in *.
-      apply Union_introl. unfold In.
-      eapply subst_rho_close_var_eff; eauto.
-    SCase "case2".
-      apply H8 with  (r:=x0); unfold In in *; simpl in *.
-      apply Union_intror. unfold In.
-      eapply subst_rho_close_var; eauto. 
+    eapply ty_sound_region_closure; try (solve [eassumption]). auto.
   Case "mu_app".   
     edestruct IHD1 as [sttym [Weak1 [TcHeap1 TcVal_mu]]]; eauto. 
     edestruct IHD2 as [sttya [Weaka [TcHeapa TcVal_arg]]]; eauto.  
     eapply ext_stores__env; eauto.  
     inversion TcVal_mu as [ | | | ? ? ? ? ? ? ?   TcRho_rho' TcEnv_env' TcExp_abs | | |] ; subst.      
     inversion TcExp_abs as [ | |  | ? ? ? ? ? ? ? ? ? ? ? ? TcExp_ec TcExp_ee | | | | | | | | | | | | | | | | | | | | | ]; subst. 
-    rewrite <- H5 in TcVal_mu. 
-    do 2 rewrite subst_rho_arrow in H5. inversion H5.
+    rewrite <- H4 in TcVal_mu. 
+    do 2 rewrite subst_rho_arrow in H4. inversion H4.
     assert (SubstEq1: subst_rho rho' tyx = subst_rho rho tya) by assumption. 
     assert (SubstEq2: subst_rho rho' tyc = subst_rho rho t) by assumption.
     rewrite <- SubstEq1 in TcVal_arg.
@@ -607,9 +563,9 @@ Proof.
     edestruct IHD2 as [sttyr [Weak2 [TcHeap2 TcVal_res]]]; eauto using update_env, ext_stores__env.
     apply update_rho. assumption. assumption. eapply extended_rho; eauto. 
     exists sttyr; intuition. 
-    rewrite subst_rho_forallrgn in H6.
-    rewrite subst_rho_forallrgn in H6.
-    inversion H6.  
+    rewrite subst_rho_forallrgn in H5.
+    rewrite subst_rho_forallrgn in H5.
+    inversion H5.  
     unfold update_R in TcVal_res. 
     simpl in TcVal_res. rewrite subst_add_comm in TcVal_res.
     SCase "abstraction body is well typed".
@@ -628,9 +584,9 @@ Proof.
       apply update_env.
       SSCase "TcEnv". apply update_env.
         SSSCase "Extended". eapply ext_stores__env; eauto.
-        SSSCase "Extended TcVal". rewrite <- H5 in TcVal_mu.  eapply ext_stores__val; eauto.
-      SSCase "TcVal". do 2 rewrite subst_rho_arrow in H5.
-          inversion H5.
+        SSSCase "Extended TcVal". rewrite <- H4 in TcVal_mu.  eapply ext_stores__val; eauto.
+      SSCase "TcVal". do 2 rewrite subst_rho_arrow in H4.
+          inversion H4.
           assert (SubstEq: subst_rho rho' tyx = subst_rho rho tya) by assumption.
           rewrite <- SubstEq in TcVal_arg.  eassumption. 
     exists sttyb. intuition.
